[sledge sem] Improve and unify treatment of Exit
Summary:
Add an argument to the Exit instruction. Update the LLVM semantics to
execute the Exit instruction and store the result in an "exited"
component of the state. (Previously it just noticed that it was stuck
about to do an Exit.)

With exiting treated uniformly, now in the proof that for every LLVM
trace, there is a llair trace that simulates it, all of the cheats
except for 1 are just cases that I haven't got to yet. However, the last
cheat is for the situation where the LLVM program gets stuck and the
llair program doesn't. For example, the following two line LLVM program
gets stuck because r2 is not assigned (ignoring for the moment the static
restriction that LLVM is in SSA form).

r1 := r2
Exit(0)

The compilation to llair omits the assignment and so we get a llair
program that doesn't get stuck:

Exit(0)

The key question is whether the static restrictions are sufficient to
ensure that no expression that might be omitted can get stuck.

Reviewed By: jberdine

Differential Revision: D17737589

fbshipit-source-id: bc6c01a1b

sledge/semantics/llvmScript.sml
@@ -90,7 +90,7 @@ Datatype:
   | Br arg label label
   | Invoke reg ty arg (targ list) label label
   | Unreachable
-  | Exit
+  | Exit arg
   (* Non-terminators *)
   | Sub reg bool bool ty arg arg
   | Extractvalue reg targ (const list)
@@ -144,7 +144,7 @@ Definition terminator_def:
   (terminator (Br _ _ _) ⇔ T) ∧
   (terminator (Invoke _ _ _ _ _ _) ⇔ T) ∧
   (terminator Unreachable ⇔ T) ∧
-  (terminator Exit ⇔ T) ∧
+  (terminator (Exit _) ⇔ T) ∧
   (terminator (Cxa_throw _ _ _) ⇔ T) ∧
   (terminator _ ⇔ F)
 End
@@ -196,7 +196,8 @@ Datatype:
        globals : glob_var |-> (num # word64);
        locals : reg |-> pv;
        stack : frame list;
-       heap : bool heap |>
+       heap : bool heap;
+       exited : int option |>
 End
 
 (* ----- Things about types ----- *)
@@ -524,6 +525,13 @@ Inductive step_instr:
   (* TODO *)
   (step_instr prog s (Invoke r t a args l1 l2) Tau s) ∧
 
+  (eval s a = Some v1 ∧
+  signed_v_to_int v1.value = Some exit_code
+   ⇒
+   step_instr prog s
+     (Exit a) Tau
+     (s with exited := Some (exit_code))) ∧
+
   (eval s a1 = Some v1 ∧
    eval s a2 = Some v2 ∧
    do_sub nuw nsw v1 v2 t = Some v3
@@ -677,6 +685,7 @@ End
 
 Inductive step:
  (get_instr p s.ip (Inl i) ∧
+  s.exited = None ∧
   step_instr p s i l s'
   ⇒
   step p s l s') ∧
@@ -693,6 +702,7 @@ Inductive step:
  * %r1 = phi [0, %l]
  *)
  (get_instr p s.ip (Inr (from_l, phis)) ∧
+  s.exited = None ∧
   map (do_phi from_l s) phis = map Some updates
   ⇒
   step p s Tau (inc_pc (s with locals := locals |++ updates)))
@@ -701,8 +711,8 @@ End
 
 Definition get_observation_def:
   get_observation prog last_s =
-    if get_instr prog last_s.ip (Inl Exit) then
-      Complete
+    if last_s.exited ≠ None then
+      Complete (THE last_s.exited)
     else if ∃s l. step prog last_s l s then
       Partial
     else
@@ -799,6 +809,7 @@ Definition is_init_state_def:
     s.ip.i = Offset 0 ∧
     s.locals = fempty ∧
     s.stack = [] ∧
+    s.exited = None ∧
     globals_ok s ∧
     heap_ok s.heap ∧
     fdom s.globals = fdom global_init ∧
